
<h2><a href="https://leetcode.com/problems/lexicographically-smallest-equivalent-string/description/">1061. Lexicographically Smallest Equivalent String</a></h2>
<h3>Medium</h3>
<hr>
<div><p>
You are given two strings of the same length s1 and s2 and a string baseStr.

We say s1[i] and s2[i] are equivalent characters.

For example, if s1 = "abc" and s2 = "cde", then we have 'a' == 'c', 'b' == 'd', and 'c' == 'e'.
Equivalent characters follow the usual rules of any equivalence relation:

Reflexivity: 'a' == 'a'.
Symmetry: 'a' == 'b' implies 'b' == 'a'.
Transitivity: 'a' == 'b' and 'b' == 'c' implies 'a' == 'c'.
For example, given the equivalency information from s1 = "abc" and s2 = "cde", "acd" and "aab" are equivalent strings of baseStr = "eed", and "aab" is the lexicographically smallest equivalent string of baseStr.

Return the lexicographically smallest equivalent string of baseStr by using the equivalency information from s1 and s2.
</p>


<p><strong>Example 1:</strong></p>
<pre><strong>Input:</strong>   s1 = "parker", s2 = "morris", baseStr = "parser"
<strong>Output:</strong> [8,6,2,4]
</pre>
<pre>
Explanation: At the beginning, the array is [1,2,3,4].
After adding 1 to nums[0], the array is [2,2,3,4], and the sum of even values is 2 + 2 + 4 = 8.
After adding -3 to nums[1], the array is [2,-1,3,4], and the sum of even values is 2 + 4 = 6.
After adding -4 to nums[0], the array is [-2,-1,3,4], and the sum of even values is -2 + 4 = 2.
After adding 2 to nums[3], the array is [-2,-1,3,6], and the sum of even values is -2 + 6 = 4.
  </pre>
  
Example 2:

Input: nums = [1], queries = [[4,0]]
Output: [0]
 

Constraints:
<pre>
1 <= nums.length <= 104
-104 <= nums[i] <= 104
1 <= queries.length <= 104
-104 <= vali <= 104
0 <= indexi < nums.length
</pre>
<hr>
 <h2><strong><b>Solution</b></strong></h2>
 <br>
 <pre>
 
          class Solution {
          public:
              vector<int> sumEvenAfterQueries(vector<int>& nums, vector<vector<int>>& q) {
                  int ans=0;
                  for(int i=0;i<nums.size();i++)
                  {
                      if(nums[i]%2==0) ans+=nums[i];
                  }
                  vector<int> v;
                  for(int i=0;i<q.size();i++)
                  {
                      int val=q[i][0],ind=q[i][1];
                      if(nums[ind]%2==0) ans-=nums[ind];
                      nums[ind]+=val;
                      if(nums[ind]%2==0) ans+=nums[ind];
                      v.push_back(ans);
                  }
                  return v;
              }
          };
          
 </pre>

